code/k256/Hacl.EC.K256.fst
@@ -1,0 +1,259 @@
+module Hacl.EC.K256
+
+open FStar.HyperStack
+open FStar.HyperStack.ST
+open FStar.Mul
+
+open Lib.IntTypes
+open Lib.Buffer
+
+module ST = FStar.HyperStack.ST
+module BSeq = Lib.ByteSequence
+module LSeq = Lib.Sequence
+
+module S = Spec.K256
+
+module F = Hacl.K256.Field
+module Q = Hacl.K256.Scalar
+module FI = Hacl.Impl.K256.Finv
+module QI = Hacl.Impl.K256.Qinv
+
+module P = Hacl.Impl.K256.Point
+module PA = Hacl.Impl.K256.PointAdd
+module PD = Hacl.Impl.K256.PointDouble
+module PM = Hacl.Impl.K256.PointMul
+
+module BL = Hacl.Spec.K256.Field52.Lemmas
+module BB = Hacl.Bignum.Base
+
+#set-options "--z3rlimit 50 --fuel 0 --ifuel 0"
+
+///  Finite field arithmetic
+
+val mk_felem_zero: f:F.felem -> Stack unit
+  (requires fun h -> live h f)
+  (ensures  fun h0 _ h1 -> modifies (loc f) h0 h1 /\
+    F.inv_lazy_reduced2 h1 f /\ F.feval h1 f == S.zero)
+
+let mk_felem_zero f =
+  Math.Lemmas.small_mod S.zero S.prime;
+  F.set_zero f
+
+
+val mk_felem_one: f:F.felem -> Stack unit
+  (requires fun h -> live h f)
+  (ensures  fun h0 _ h1 -> modifies (loc f) h0 h1 /\
+    F.inv_lazy_reduced2 h1 f /\ F.feval h1 f == S.one)
+
+let mk_felem_one f =
+  Math.Lemmas.small_mod S.one S.prime;
+  F.set_one f
+
+
+val felem_add (a b out:F.felem) : Stack unit
+  (requires fun h ->
+    live h a /\ live h b /\ live h out /\
+    eq_or_disjoint out a /\ eq_or_disjoint out b /\ eq_or_disjoint a b /\
+    F.inv_lazy_reduced2 h a /\ F.inv_lazy_reduced2 h b)
+  (ensures  fun h0 _ h1 -> modifies (loc out) h0 h1 /\
+    F.inv_lazy_reduced2 h1 out /\
+    F.feval h1 out == S.fadd (F.feval h0 a) (F.feval h0 b))
+
+let felem_add a b out =
+  let h0 = ST.get () in
+  BL.fadd5_lemma (1,1,1,1,2) (1,1,1,1,2) (F.as_felem5 h0 a) (F.as_felem5 h0 b);
+  F.fadd out a b;
+  let h1 = ST.get () in
+  assert (F.felem_fits5 (F.as_felem5 h1 out) (2,2,2,2,4));
+  BL.normalize_weak5_lemma (2,2,2,2,4) (F.as_felem5 h1 out);
+  F.fnormalize_weak out out
+
+
+val felem_sub (a b out:F.felem) : Stack unit
+  (requires fun h ->
+    live h a /\ live h b /\ live h out /\
+    eq_or_disjoint out a /\ eq_or_disjoint out b /\ eq_or_disjoint a b /\
+    F.inv_lazy_reduced2 h a /\ F.inv_lazy_reduced2 h b)
+  (ensures  fun h0 _ h1 -> modifies (loc out) h0 h1 /\
+    F.inv_lazy_reduced2 h1 out /\
+    F.feval h1 out == S.fsub (F.feval h0 a) (F.feval h0 b))
+
+let felem_sub a b out =
+  let h0 = ST.get () in
+  BL.fsub5_lemma (1,1,1,1,2) (1,1,1,1,2) (F.as_felem5 h0 a) (F.as_felem5 h0 b) (u64 2);
+  F.fsub out a b (u64 2);
+  let h1 = ST.get () in
+  assert (F.felem_fits5 (F.as_felem5 h1 out) (5,5,5,5,6));
+  BL.normalize_weak5_lemma (5,5,5,5,6) (F.as_felem5 h1 out);
+  F.fnormalize_weak out out
+
+
+val felem_mul (a b out:F.felem) : Stack unit
+  (requires fun h ->
+    live h a /\ live h b /\ live h out /\
+    eq_or_disjoint out a /\ eq_or_disjoint out b /\ eq_or_disjoint a b /\
+    F.inv_lazy_reduced2 h a /\ F.inv_lazy_reduced2 h b)
+  (ensures  fun h0 _ h1 -> modifies (loc out) h0 h1 /\
+    F.inv_lazy_reduced2 h1 out /\
+    F.feval h1 out == S.fmul (F.feval h0 a) (F.feval h0 b))
+
+let felem_mul a b out =
+  F.fmul out a b
+
+
+val felem_sqr (a out:F.felem) : Stack unit
+  (requires fun h ->
+    live h a /\ live h out /\ eq_or_disjoint out a /\
+    F.inv_lazy_reduced2 h a)
+  (ensures  fun h0 _ h1 -> modifies (loc out) h0 h1 /\
+    F.inv_lazy_reduced2 h1 out /\
+    F.feval h1 out == S.fmul (F.feval h0 a) (F.feval h0 a))
+
+let felem_sqr a out =
+  F.fsqr out a
+
+
+val felem_inv (a out:F.felem) : Stack unit
+  (requires fun h ->
+    live h a /\ live h out /\ disjoint a out /\
+    F.inv_lazy_reduced2 h a)
+  (ensures  fun h0 _ h1 -> modifies (loc out) h0 h1 /\
+    F.inv_lazy_reduced2 h1 out /\
+    F.feval h1 out == S.finv (F.feval h0 a))
+
+let felem_inv a out =
+  FI.finv out a
+
+
+val felem_load: b:lbuffer uint8 32ul -> out:F.felem -> Stack unit
+  (requires fun h -> live h b /\ live h out /\ disjoint b out)
+  (ensures  fun h0 _ h1 -> modifies (loc out) h0 h1 /\
+    F.inv_lazy_reduced2 h1 out /\
+    F.feval h1 out == BSeq.nat_from_bytes_be (as_seq h0 b) % S.prime)
+
+let felem_load b out =
+  F.load_felem out b
+
+
+val felem_store: a:F.felem -> out:lbuffer uint8 32ul -> Stack unit
+  (requires fun h ->
+    live h a /\ live h out /\ disjoint a out /\
+    F.inv_lazy_reduced2 h a)
+  (ensures  fun h0 _ h1 -> modifies (loc out) h0 h1 /\
+    as_seq h1 out == BSeq.nat_to_bytes_be 32 (F.feval h0 a))
+
+let felem_store a out =
+  push_frame ();
+  let tmp = F.create_felem () in
+  let h0 = ST.get () in
+  BL.normalize5_lemma (1,1,1,1,2) (F.as_felem5 h0 a);
+  F.fnormalize tmp a;
+  F.store_felem out tmp;
+  pop_frame ()
+
+
+///  Elliptic curve operations
+
+val mk_point_at_inf: p:P.point -> Stack unit
+  (requires fun h -> live h p)
+  (ensures  fun h0 _ h1 -> modifies (loc p) h0 h1 /\
+    P.point_inv h1 p /\ P.point_eval h1 p == S.point_at_inf)
+
+let mk_point_at_inf p =
+  PM.make_point_at_inf p
+
+
+val mk_base_point: p:P.point -> Stack unit
+  (requires fun h -> live h p)
+  (ensures  fun h0 _ h1 -> modifies (loc p) h0 h1 /\
+    P.point_inv h1 p /\ P.point_eval h1 p == S.g)
+
+let mk_base_point p =
+  PM.make_g p
+
+
+val point_negate (p out:P.point) : Stack unit
+  (requires fun h ->
+    live h out /\ live h p /\ eq_or_disjoint out p /\
+    P.point_inv h p)
+  (ensures  fun h0 _ h1 -> modifies (loc out) h0 h1 /\
+    P.point_inv h1 out /\
+    P.point_eval h1 out == S.point_negate (P.point_eval h0 p))
+
+let point_negate p out =
+  P.point_negate out p
+
+
+val point_add (p q out:P.point) : Stack unit
+  (requires fun h ->
+    live h out /\ live h p /\ live h q /\
+    eq_or_disjoint p out /\ eq_or_disjoint q out /\ eq_or_disjoint p q /\
+    P.point_inv h p /\ P.point_inv h q)
+  (ensures  fun h0 _ h1 -> modifies (loc out) h0 h1 /\
+    P.point_inv h1 out /\
+    P.point_eval h1 out == S.point_add (P.point_eval h0 p) (P.point_eval h0 q))
+
+let point_add p q out =
+  PA.point_add out p q
+
+
+val point_double (p out:P.point) : Stack unit
+  (requires fun h ->
+    live h out /\ live h p /\ eq_or_disjoint p out /\
+    P.point_inv h p)
+  (ensures  fun h0 _ h1 -> modifies (loc out) h0 h1 /\
+    P.point_inv h1 out /\ P.point_eval h1 out == S.point_double (P.point_eval h0 p))
+
+let point_double p out =
+  PD.point_double out p
+
+
+val point_mul: scalar:lbuffer uint8 32ul -> p:P.point -> out:P.point -> Stack unit
+  (requires fun h ->
+    live h scalar /\ live h p /\ live h out /\
+    disjoint out p /\ disjoint out scalar /\ disjoint p scalar /\
+    P.point_inv h p /\
+    BSeq.nat_from_bytes_be (as_seq h scalar) < S.q)
+  (ensures  fun h0 _ h1 -> modifies (loc out) h0 h1 /\
+    P.point_inv h1 out /\
+    P.point_eval h1 out == S.point_mul (BSeq.nat_from_bytes_be (as_seq h0 scalar)) (P.point_eval h0 p))
+
+let point_mul scalar p out =
+  push_frame ();
+  let scalar_q = Q.create_qelem () in
+  Q.load_qelem scalar_q scalar;
+  PM.point_mul out scalar_q p;
+  pop_frame ()
+
+
+val point_eq (p q:P.point) : Stack bool
+  (requires fun h ->
+    live h p /\ live h q /\ eq_or_disjoint p q /\
+    P.point_inv h p /\ P.point_inv h q)
+  (ensures  fun h0 z h1 -> modifies0 h0 h1 /\
+    (z <==> S.point_equal (P.point_eval h0 p) (P.point_eval h0 q)))
+
+let point_eq p q =
+  P.point_eq p q
+
+
+val point_compress: p:P.point -> out:lbuffer uint8 33ul -> Stack unit
+  (requires fun h ->
+    live h out /\ live h p /\ disjoint p out /\
+    P.point_inv h p)
+  (ensures  fun h0 _ h1 -> modifies (loc out) h0 h1 /\
+    as_seq h1 out == S.point_compress (P.point_eval h0 p))
+
+let point_compress p out =
+  P.point_compress_vartime out p
+
+
+val point_decompress: s:lbuffer uint8 33ul -> out:P.point -> Stack bool
+  (requires fun h ->
+    live h out /\ live h s /\ disjoint out s)
+  (ensures  fun h0 b h1 -> modifies (loc out) h0 h1 /\
+    (b <==> Some? (S.point_decompress (as_seq h0 s))) /\
+    (b ==> (P.point_inv h1 out /\ P.point_eval h1 out == Some?.v (S.point_decompress (as_seq h0 s)))))
+
+let point_decompress s out =
+  P.point_decompress_vartime out s
