specs/Spec.K256.fst
@@ -169,15 +169,11 @@ let pk_uncompressed_from_raw (pk:lbytes 64) : lbytes 65 =
   concat (create 1 (u8 0x04)) pk
 
 let pk_compressed_to_raw (pk:lbytes 33) : option (lbytes 64) =
-  let pk0 = Lib.RawIntTypes.u8_to_UInt8 pk.[0] in
-  if not (pk0 = 0x02uy || pk0 = 0x03uy) then None
-  else begin
-    let pk_xb = sub pk 1 32 in
-    let is_pk_y_odd = pk0 = 0x03uy in
-    let pk_yb = recover_y_bytes pk_xb is_pk_y_odd in
-    match pk_yb with
-    | Some pk_yb -> Some (concat #_ #32 #32 pk_xb pk_yb)
-    | None -> None end
+  let pk_x = sub pk 1 32 in
+  match (aff_point_decompress pk) with
+  | Some (x, y) -> Some (concat #_ #32 #32 pk_x (nat_to_bytes_be 32 y))
+  | None -> None
+
 
 let pk_compressed_from_raw (pk:lbytes 64) : lbytes 33 =
   let pk_x = sub pk 0 32 in
